Verifica traduccion Lambda -> SKI

BracketAbstraction.Equality.fst
@@ -7,17 +7,12 @@ open Subst
 open Lam.Equality
 
 
-
-let abs_fnl (t : ski) : Lemma (fnl t ==> fnl (abstract_ski t))
-= ()
-
-
-let rec abstract_App (#n : nat) (t : nclosed_ski (n + 1)) (v : nclosed_ski n)
-: ski_eq #n (App (nclosed_abstraction (n + 1) t) v) (subst_nclosed_ski #n t v 0)
+let rec abstract_App (t v : ski)
+: ski_eq (App (abstract t) v) (subst_ski t v 0)
 = match t with
   | App t u ->
-    let abs_t = nclosed_abstraction (n + 1) t  in
-    let abs_u = nclosed_abstraction (n + 1) u  in
+    let abs_t = abstract t  in
+    let abs_u = abstract u  in
     let red_s = Red_S abs_t abs_u v in
     let hi_t = abstract_App t v in
     let hi_u = abstract_App u v in
@@ -31,18 +26,12 @@ let rec abstract_App (#n : nat) (t : nclosed_ski (n + 1)) (v : nclosed_ski n)
   | Unit -> Red_K Unit v
 
 
-let rec expand_subst (n : nat) (t : nclosed_ski (n + 1)) (v : nclosed_ski n)
-: Lemma (expand #n (subst_nclosed_ski t v 0) = subst_nclosed_ski (expand #(n + 1) t) (extend_ski #n #1 v) 0)
-= match t with
-  | App t u -> expand_subst n t v ; expand_subst n u v
-  | _ -> ()
 
-let rec subst_ski_eq (#n : nat) (#t #u: nclosed_ski (n + 1)) (eq : ski_eq t u)
-                     (v : nclosed_ski n)
-                     
-: Tot (ski_eq #n (subst_nclosed_ski t v 0) (subst_nclosed_ski u v 0))
+let rec subst_ski_eq (#t #u: ski) (eq : ski_eq t u)
+                     (v : ski)
+: Tot (ski_eq (subst_ski t v 0) (subst_ski u v 0))
       (decreases eq)
-= let sub t = subst_nclosed_ski t v 0 in
+= let sub t = subst_ski t v 0 in
   match eq with
   | Refl _ -> Refl _
   | Symm eq -> Symm (subst_ski_eq eq v)
@@ -51,69 +40,112 @@ let rec subst_ski_eq (#n : nat) (#t #u: nclosed_ski (n + 1)) (eq : ski_eq t u)
   | Red_S f g x -> Red_S (sub f) (sub g) (sub x)
   | Red_K x y -> Red_K (sub x) (sub y)
   | Red_I x -> Red_I (sub x)
-  | Zeta eq ->
-    expand_subst n t v ;
-    expand_subst n u v ;
-    Zeta (subst_ski_eq #(n + 1) eq (extend_ski #n #1 v))
+  | Zeta ext ->
+    let t' = subst_ski t v 0 in
+    let u' = subst_ski u v 0 in
+    let ext' (i : nat {not_free i t' /\ not_free i u'})
+    : ski_eq (App t' (Var i)) (App u' (Var i))
+    = not_free_subst_ski t v i ;
+      not_free_subst_ski u v i ;
+      subst_ski_eq (ext (i + 1)) v in
+    Zeta ext' 
 
+let app2 (t u v : ski) : ski = App (App t u) v
+let app3 (t u v w : ski) : ski = App (app2 t u v) w
 
+let ( @ ) (t u : ski) : ski = App t u
 
-let ( @ ) (#n : nat) (t u : nclosed_ski n) : nclosed_ski n = App t u
+let abstract_S_ski_eq (f g x y : ski)
+: ski_eq (((S @ ((S @ ((S @ (K @ S)) @ f)) @ g)) @ x) @ y)
+         (((S @ ((S @ f) @ x)) @ ((S @ g) @ x)) @ y)
+= let red_1 = Red_S ((S  @ ((S @ (K @ S)) @ f)) @ g) x y in
+  let red_2 = Red_S (App (App S (App K S)) f) g y in
+  let red_2 = Red_S ((S @ (K @ S)) @ f) g y in
+  let red_3 = Red_S (K @ S) f y in
+  let red_4 = Red_K S y in
+  let app_2 = App_eq red_2 (Refl (x @ y)) in
+  let app_3_1 = App_eq red_3 (Refl (g @ y)) in
+  let app_3_2 = App_eq app_3_1 (Refl (x @ y)) in
+  let app_4_1 = App_eq red_4 (Refl (f @ y)) in
+  let app_4_2 = App_eq app_4_1 (Refl (g @ y)) in 
+  let app_4_3 = App_eq app_4_2 (Refl (x @ y)) in
+  let red_5 = Red_S (f @ y) (g @ y) (x @ y) in
+  let lhs = Tran (Tran (Tran (Tran red_1 app_2) app_3_2) app_4_3) red_5 in
+  let red_1 = Red_S ((S @ f) @ x) ((S @ g) @ x) y in
+  let redl = Red_S f x y in
+  let redr = Red_S g x y in
+  let rhs = Tran red_1 (App_eq redl redr) in
+  Tran lhs (Symm rhs)
 
+let abstract_K_ski_eq (x y z : ski)
+: ski_eq (((S @ ((S @ (K @ K)) @ x)) @ y) @ z)
+         (x @ z)
+= let red_S_1 = Red_S ((S @ (K @ K)) @ x) y z in
+  let red_S_2 = Red_S (K @ K) x z in
+  let red_K_1 = Red_K K z in
+  let red_K_2 = Red_K (x @ z) (y @ z) in
+  let app_1 = App_eq red_S_2 (Refl (y @ z)) in
+  let app_2 = App_eq (App_eq red_K_1 (Refl _)) (Refl _) in
+  let lhs_1 = Tran red_S_1 app_1 in
+  let lhs_2 = Tran lhs_1 app_2 in
+  Tran lhs_2 red_K_2
 
-let rec abstract_ski_eq (n : pos) (#t #u : nclosed_ski n) (t_eq_u : ski_eq t u)
-: Tot (ski_eq (nclosed_abstraction n t) (nclosed_abstraction n u))
+let abstract_I_ski_eq (x y : ski)
+: ski_eq (((S @ (K @ I)) @ x) @ y)
+         (x @ y)
+= let red_S = Red_S (K @ I) x y in
+  let red_K = Red_K I y in
+  let red_I = Red_I (x @ y) in
+  let app = App_eq red_K (Refl _) in
+  Tran (Tran red_S app) red_I
+
+let rec abstract_ski_eq (#t #u : ski) (t_eq_u : ski_eq t u)
+: Tot (ski_eq (abstract t) (abstract u))
       (decreases t_eq_u)
 = match t_eq_u with
-| Red_S f g x -> admit ()
-// let f' : nclosed_ski n = extend_ski #(n - 1) #1 (nclosed_abstraction n f) in
-// let g' : nclosed_ski n = extend_ski #(n - 1) #1 (nclosed_abstraction n g) in
-// let x' : nclosed_ski n = extend_ski #(n - 1) #1 (nclosed_abstraction n x) in
-// let y : nclosed_ski n = Var (n - 1) in
-// let k  : nclosed_ski n = ((S @ ((S @ (K @ S)) @ f')) @ g') in 
-// let red_1 = Red_S k x' y in
-// let red_2 = Red_S (App (App S (App K S)) f') g' y in
-// let red_3 = Red_S (App K S) f' y in
-// let red_4 = Red_K S y in
-// let app_2 = App_eq red_2 (Refl (App x' y)) in
-// let app_3_1 = App_eq red_3 (Refl (App g' y)) in
-// let app_3_2 = App_eq app_3_1 (Refl (App x' y)) in
-// let app_4_1 = App_eq red_4 (Refl (App f' y)) in
-// let app_4_2 = App_eq app_4_1 (Refl (App g' y)) in 
-// let app_4_3 = App_eq app_4_2 (Refl (App x' y)) in
-// let red_5 = Red_S #n (App f' y) (App g' y) (App x' y) in
-// let lhs = Tran (Tran (Tran (Tran red_1 app_2) app_3_2) app_4_3) red_5 in
-// let red_1 = Red_S ((S @ f') @ x') ((S @ g') @ x') y in
-// let redl = Red_S f' x' y in
-// let redr = Red_S g' x' y in
-// let rhs = Tran red_1 (App_eq redl redr) in
-// assert (t = ((S @ f) @ g) @ x) ;
-// assert (abstract g = g') ;
-// Zeta (Tran lhs (Symm rhs))
-| Red_K x y ->
-let x' : nclosed_ski n = extend_ski #(n - 1) #1 (nclosed_abstraction n x) in
-let y' : nclosed_ski n = extend_ski #(n - 1) #1 (nclosed_abstraction n y) in
-let z : nclosed_ski n = Var (n - 1) in
-admit ()
-| Red_I x ->
-let x' : nclosed_ski n = extend_ski #(n - 1) #1 (nclosed_abstraction n x) in
-let y : nclosed_ski n = Var (n - 1) in
-let red_S = Red_S (K @ I) x' y in
-let red_K = Red_K I y in
-let app = App_eq (red_K) (Refl (x' @ y)) in
-let red_I = Red_I (x' @ y) in
-Zeta (Tran (Tran red_S app) red_I)
-| App_eq eq1 eq2 -> App_eq (App_eq (Refl S) (abstract_ski_eq n eq1)) (abstract_ski_eq n eq2)
 | Refl t -> Refl _
-| Symm eq -> Symm (abstract_ski_eq n eq)
-| Tran eq1 eq2 -> Tran (abstract_ski_eq n eq1) (abstract_ski_eq n eq2)
-| Zeta eq -> admit ()
+| Symm eq -> Symm (abstract_ski_eq eq)
+| Tran eq1 eq2 -> Tran (abstract_ski_eq eq1) (abstract_ski_eq eq2)
+| App_eq eq1 eq2 -> App_eq (App_eq (Refl S) (abstract_ski_eq eq1)) (abstract_ski_eq eq2)
+| Zeta ext ->
+  let t' = abstract t in
+  let u' = abstract u in
+  let ext' (i : nat)
+  : ski_eq (App t' (Var i)) (App u' (Var i))
+  = let t'' = subst_ski t (Var i) 0 in
+    let u'' = subst_ski u (Var i) 0 in
+    let abs_app_t = abstract_App t (Var i) in
+    let abs_app_u = abstract_App u (Var i) in
+    let ext'' (j : nat {not_free j t'' && not_free j u''})
+    = not_free_subst_ski t (Var i) j ; 
+      not_free_subst_ski u (Var i) j ;
+      subst_ski_eq (ext (j + 1)) (Var i)
+    in Tran (Tran abs_app_t (Zeta ext'')) (Symm abs_app_u)
+  in Zeta ext'
+| Red_S f g x ->
+  let f' : ski= abstract f in
+  let g' : ski= abstract g in
+  let x' : ski= abstract x in
+  let ext (i : nat {not_free i f' && not_free i g' && not_free i x'})
+  = abstract_S_ski_eq f' g' x' (Var i)
+  in Zeta ext
+| Red_K x y ->
+  let x' : ski = abstract x in
+  let y' : ski = abstract y in
+  let ext (i : nat {not_free i x' && not_free i y'})
+  = abstract_K_ski_eq x' y' (Var i)
+  in Zeta ext
+| Red_I x ->
+let x' : ski = abstract x in
+let ext (i : nat {not_free i x'})
+= abstract_I_ski_eq x' (Var i)
+in Zeta ext
 
 
 
 
 let rec shift_abs (n : nat) (t : ski)
-: Lemma (shiftn n (abstract t) = abstract (shiftn (n + 1) t))
+: Lemma (shiftn n (abstract t) = abstract (shiftn_ski (n + 1) t))
 = match t with
   | App t u -> shift_abs n t ; shift_abs n u 
   | _ -> ()
@@ -128,73 +160,71 @@ let rec shift_bracket (i : nat) (t : lam)
   | App t u -> shift_bracket i t ; shift_bracket i u
   | _ -> ()
 
-let ski_eq_S_K (#n : nat) (t u : nclosed_ski n)
-: ski_eq #n (App (App S (App K t)) (App K u)) (App K (App t u))
-= let red_S = Red_S (extend_ski (App K t)) (extend_ski (App K u)) (Var n) in
-  let red_K_l = Red_K #(n + 1) (extend_ski t) (Var n) in
-  let red_K_r = Red_K #(n + 1) (extend_ski u) (Var n) in
-  let red_K_app = App_eq red_K_l red_K_r in
-  let lhs = Tran red_S red_K_app in
-  let red_K = Red_K #(n + 1) (extend_ski (App t u)) (Var n) in
-  let rhs = Symm red_K in
-  Zeta (Tran lhs rhs)
+let ski_eq_S_K (t u : ski)
+: ski_eq (App (App S (App K t)) (App K u)) (App K (App t u))
+= let ext (i : nat {not_free i t && not_free i u})
+  = let red_S = Red_S (App K t) (App K u) (Var i) in
+    let red_K_l = Red_K t (Var i) in
+    let red_K_r = Red_K u (Var i) in
+    let red_K_app = App_eq red_K_l red_K_r in
+    let lhs = Tran red_S red_K_app in
+    let red_K = Red_K (App t u) (Var i) in
+    let rhs = Symm red_K in
+    Tran lhs rhs
+  in Zeta ext
 
-let rec ski_eq_abstract (#n : nat) (t : nclosed_ski n)
-: ski_eq #n (nclosed_abstraction (n + 1) (shift_nclosed_ski t)) (App K t)
+let rec ski_eq_abstract (t : ski)
+: ski_eq (abstract (shift_ski t)) (App K t)
 = match t with
   | App t u ->
-    let hi_t = ski_eq_abstract #n t in
-    let hi_u = ski_eq_abstract #n u in
+    let hi_t = ski_eq_abstract t in
+    let hi_u = ski_eq_abstract u in
     let hi_appl = App_eq (Refl S) (hi_t) in
     let hi_app = App_eq (hi_appl) (hi_u) in
-    let eq_SK = ski_eq_S_K #n t u in
+    let eq_SK = ski_eq_S_K t u in
     Tran hi_app eq_SK
   | _ -> Refl _
 
-let rec subst_abstract (#n : nat) (t : nclosed_ski (n + 2)) (v : nclosed_ski n) (i : nat {i <= n})
-: ski_eq #n (nclosed_abstraction (n + 1) (subst_nclosed_ski t (shift_nclosed_ski #n v) (i + 1)))
-            (subst_nclosed_ski (nclosed_abstraction (n + 2) t) v i)
+let rec subst_abstract (t : ski) (v : ski) (i : nat)
+: ski_eq (abstract (subst_ski t (shift_ski v) (i + 1)))
+         (subst_ski (abstract t) v i)
 = match t with
   | App t u ->
     App_eq (App_eq (Refl S) (subst_abstract t v i)) (subst_abstract u v i)  
   | Var j ->
     if j = i + 1
-    then ski_eq_abstract #n v
+    then ski_eq_abstract v
     else Refl _
   | _ -> Refl _
 
 
-let rec subst_bracket (#n : nat) (t : nclosed_lam (n + 1)) (v : nclosed_lam n) (i : nat {i <= n})
-: Tot
-    (ski_eq #n
-      (nclosed_bracket_abstraction n (subst_nclosed_lam t v i))
-      (subst_nclosed_ski (nclosed_bracket_abstraction (n + 1) t) (nclosed_bracket_abstraction n v) i))
-    (decreases t)
+let rec subst_bracket (t : lam) (v : lam) (i : nat)
+: Tot (ski_eq (bracket_abstraction (subst_lam t v i))
+              (subst_ski (bracket_abstraction t) (bracket_abstraction v) i))
+      (decreases t)
 = match t with
   | Abs _ t ->
-    // TODO comentar esto
     shift_bracket 0 v ;
-    let hi = subst_bracket #(n + 1) t (shift_nclosed_lam v) (i + 1) in
-    let hi = abstract_ski_eq (n + 1) _ _ hi in 
-    let bracket_t = nclosed_bracket_abstraction (n + 2) t in
-    let bracket_v = nclosed_bracket_abstraction n v in
+    let hi = subst_bracket t (shift_lam v) (i + 1) in
+    let hi = abstract_ski_eq hi in 
+    let bracket_t = bracket_abstraction t in
+    let bracket_v = bracket_abstraction v in
     let subst_abstract_eq = subst_abstract bracket_t bracket_v i in
     Tran hi subst_abstract_eq
   | App t u -> App_eq (subst_bracket t v i) (subst_bracket u v i)
   | _ -> Refl _
 
 
-let rec step_preserves_eq (#n : nat) (#t #u : nclosed_lam n) (st : step t u)
-: ski_eq #n (nclosed_bracket_abstraction n t) (nclosed_bracket_abstraction n u) =
+let rec step_preserves_eq (#t #u : lam) (st : step t u)
+: ski_eq (bracket_abstraction t) (bracket_abstraction u) =
   match st with
   | AppL st_t u -> 
-    nclosed_step_impl n st ;
-    App_eq (step_preserves_eq st_t) (Refl (nclosed_bracket_abstraction n u))
-  | AppR t st_u -> admit ()
+    App_eq (step_preserves_eq st_t) (Refl (bracket_abstraction u))
+  | AppR t st_u ->
+    App_eq (Refl (bracket_abstraction t)) (step_preserves_eq st_u)
   | Beta _ t u ->
-    nclosed_step_impl n st ;
-    let bracket_t = nclosed_bracket_abstraction (n + 1) t in
-    let bracket_u = nclosed_bracket_abstraction n u in
-    Tran (abstract_App #n bracket_t bracket_u) (Symm (subst_bracket #n t u 0))
-  | Down _ st -> admit ()
+    let bracket_t = bracket_abstraction t in
+    let bracket_u = bracket_abstraction u in
+    Tran (abstract_App bracket_t bracket_u) (Symm (subst_bracket t u 0))
+  | Down _ st -> abstract_ski_eq (step_preserves_eq st)
   
